 흡수 항등식: $\binom{r}{k}=\frac{r}{k}\binom{r-1}{k-1}$, 정수 $k\neq0$
 
 덧셈 공식: $\binom{r}{k}=\binom{r-1}{k}+\binom{r-1}{k-1}$
 
 $\binom{r}{k}=(-1)^k\binom{k-r-1}{k}$
 
 $\binom{r}{m}\binom{m}{k}=\binom{r}{k}\binom{r-k}{m-k}$

$\sum_{k\le n}\binom{r+k}{k}=\binom{r+n+1}{n}$, 정수 $n$

$\sum_{0\le k\le n}\binom{k}{m}=\binom{n+1}{m+1}$, 정수 $m,n\ge0$

Vandermonde's Identity: $\binom{m+n}{r}=\sum_{k=0}^r\binom{m}{k}\binom{n}{r-k}$\\
m=n, r=n을 대입하면 $\binom{2n}{n}=\sum\limits_{k=0}^n\binom{n}{k}\binom{n}{n-k}=\sum\limits_{k=0}^n\binom{n}{k}^2$

$\sum_k\binom{r}{m+k}\binom{s}{n-k}=\binom{r+s}{m+n}$, 정수 $m, n$

$\sum_k\binom{l}{m+k}\binom{s}{n+k}=\binom{l+s}{l-m+n}$, 정수 $l\ge0$, 정수 m, n

$\sum_k\binom{l}{m+k}\binom{s+k}{n}(-1)^k=(-1)^{l+m}\binom{s-m}{n-l}$, 정수 $l\ge0$, 정수 m, n

$\sum_{k\le l}\binom{l-k}{m}\binom{s}{k-n}(-1)^k=(-1)^{l+m}\binom{s-m-1}{l-m-n}$, 정수 $l,m,n\ge0$

$\sum_{-q\le k\le l}\binom{l-k}{m}\binom{q+k}{n}=\binom{l+q+1}{m+n+1}$, 정수 $m,n\ge0$, 정수 $l+q\ge0$